Almost full proof of poly, still small admit

compiler/proof_vec/equiv_poly1305_avx.ec
@@ -35,6 +35,16 @@ hint simplify (Array10.get_set_eqE, Array10.get_set_neqE)@0.
 
 hint simplify (iota0, iotaS_minus)@0.
 
+axiom nosmt W64_addw0 (w:W64.t) : w + W64.of_uint 0 = w. 
+axiom nosmt W64_addwA (x y z:W64.t) : x + (y + z) = x + y + z.
+axiom nosmt W64_addi x y : W64.of_uint x + W64.of_uint y = W64.of_uint (x + y).
+axiom nosmt W64_subi x y : W64.of_uint x - W64.of_uint y = W64.of_uint (x - y).
+axiom nosmt W64_shr_add i j (w:W64.t) : 0 <= i => 0 <= j => (* i + j <= 64 => *) w `>>>` i `>>>`j = w `>>>` (i+j).
+
+axiom W64_shr_or i (w1 w2 :W64.t) : (w1 `|` w2) `>>>` i = (w1 `>>>`i) `|` (w2 `>>>`i).
+axiom W64_shr_64 i (w:W64.t) : 64 <= i => w `>>>` i = W64.zeros.
+axiom W64_or0w w : W64.zeros `|` w = w.
+
 (* ------------------------------------------------------------------------------ *)
 (* AVX-5x and its optimized version AVX-5xp                                       *)
 (* ------------------------------------------------------------------------------ *)
@@ -60,6 +70,9 @@ qed.
 equiv amd64_amd64_pr_load : Poly1305_amd64_5x.M.load ~ Poly1305_amd64_5xPR.M.load :
    ={global_mem, in_0} ==> ={res}.
 proof. sim. qed.
+
+axiom W64_subaddA (x y z:W64.t) : x - (y + z) = (x - y) + z.
+axiom W64_addsubA (x y z:W64.t) : x + (y - z) = (x + y) - z.
 
 equiv poly1305_amd64_amd64_pr : 
   Poly1305_amd64_5x.M.poly1305 ~ Poly1305_amd64_5xPR.M.poly1305 :
@@ -90,7 +103,8 @@ proof.
       (={global_mem, in_0, s_r2, s_r2x5} ==> ={in_0, x0, x1, y0, y1})=> //.
     + by move=> &m1 &m2 />; exists global_mem{m2} in_0{m2} s_r2{m2} s_r2x5{m2}.
     + do !(wp;call (_: ={global_mem, in_0} ==> ={res}); 1: by sim); skip => />.
-      admit. (* Simple arithmetic stuff *)
+      move=> &m1. 
+      by rewrite -!W64_addsubA W64_subi -!W64_addwA !W64_addi.
     swap{1} 3 -1; do !(wp; call amd64_amd64_pr_load); auto => />.
 
   (* remaining_blocks *)
@@ -118,9 +132,10 @@ proof.
       ( ={global_mem, hx, hy, in_0, s_r4, s_r4x5, s_r2, s_r2x5} ==> ={in_0, hy, y1, y0, x1, x0} )   
       ( ={global_mem, hx, hy, in_0, s_r4, s_r4x5, s_r2, s_r2x5} ==> ={in_0, hy, y1, y0, x1, x0} ) => //.
     + by move=> &m1 &m2 />; exists global_mem{m2} hx{m2} hy{m2} in_0{m2} s_r2{m2} s_r2x5{m2} s_r4{m2} s_r4x5{m2}.
+    move=> />.
     + do !(wp;call (_: ={global_mem, in_0} ==> ={res}); 1: by sim); wp; skip => />.
-      admit. (* Simple arithmetic stuff *)
-    swap{1} 3 -1; do !(wp; call amd64_amd64_pr_load); auto => />.
+      by rewrite -!W64_addsubA W64_subi -!W64_addwA !W64_addi.
+    by swap{1} 3 -1; do !(wp; call amd64_amd64_pr_load); auto => />.
 
   (* final_mul *)
   proc=> /=.
@@ -166,10 +181,10 @@ op wf5 (z : W64.t Array5.t) =
    bounded 27 z.[4].
 
 op wf4 (z : W64.t Array4.t) = 
-   bounded 31 z.[0] /\
-   bounded 31 z.[1] /\
-   bounded 31 z.[2] /\
-   bounded 31 z.[3].
+   bounded 30 z.[0] /\
+   bounded 30 z.[1] /\
+   bounded 30 z.[2] /\
+   bounded 30 z.[3].
 
 axiom bounded_add i x y : 0 < i => bounded (i-1) x => bounded (i-1) y => bounded i (x + y).
 axiom bounded_and i x y : bounded i x \/ bounded i y => bounded i (x `&` y).
@@ -194,16 +209,21 @@ proof.
   by apply bounded_and;right;rewrite boundedE. 
 qed.
 
-lemma bounded_mul5 i w : bounded (i-4) w => bounded i (w * (W64.of_uint 5)).
+lemma bounded_and_2p32 i w : 32 <= i => bounded i (w `&` (W64.of_uint 4294967295)).
+  move=> h; apply (bounded_weak 32); 1: done.
+  by apply bounded_and;right;rewrite boundedE. 
+qed.
+
+lemma bounded_mul5 i w : bounded (i-3) w => bounded i (w * (W64.of_uint 5)).
 proof.
-  move=> h; have -> : i = (i - 4) + 4 by ring.
+  move=> h; have -> : i = (i - 3) + 3 by ring.
   by apply bounded_mul => //; rewrite boundedE.
 qed.
 
 hoare carry_reduceWF : Poly1305_amd64_5xPR.M.carry_reduce : true ==> wf5 res.
 proof.
   proc; wp; skip; rewrite /wf5 => &m1 &m2 /=.
-  smt (bounded_and_2p26 bounded_add bounded_shr bounded_mul5 bounded_w64).
+  smt (bounded_and_2p26 bounded_and_2p32 bounded_add bounded_shr bounded_mul5 bounded_w64).
 qed.
 
 equiv carry_reduceP : Poly1305_amd64_5xPR.M.carry_reduce ~ Poly1305_avx_5x.M.carry_reduce : 
@@ -217,8 +237,9 @@ axiom pack_mulu_32 w1 w2 :
   pack_2u32 (W32.mulu w1 w2) = (zeroext_32_64 w1) * (zeroext_32_64 w2).
 
 hint simplify pack_mulu_32.
+search zeroext_32_64.
 
-axiom zeroext_bounded w : bounded 32 w => zeroext_32_64 (unpack_2u32 w).`1 = w.
+axiom zeroext_and2p32 w : zeroext_32_64 (unpack_2u32 w).`1 = w `&` W64.of_uint 4294967295.
 
 lemma zeroext_of_uint i : zeroext_32_64 (W32.of_uint i) = W64.of_uint (i %% W32.modulus).
 proof. by rewrite zeroext_32_64E. qed.
@@ -232,7 +253,12 @@ lemma VPAND_128_64_l w1 w2 :
      pack_2u64(w1.`1 `&` (unpack_2u64 w2).`1, w1.`2 `&` (unpack_2u64 w2).`2).
 proof. by rewrite -(pack_unpack_2u64 w2) VPAND_128_64. qed.
 
-hint simplify VPAND_128_64_l@1.
+lemma VPOR_128_64_l w1 w2 : 
+   pack_2u64 w1 `|` w2 = 
+     pack_2u64(w1.`1 `|` (unpack_2u64 w2).`1, w1.`2 `|` (unpack_2u64 w2).`2).
+proof. by rewrite -(pack_unpack_2u64 w2) VPOR_128_64. qed.
+
+hint simplify (VPAND_128_64_l, VPOR_128_64_l)@1.
 
 equiv carry_reduce_u128P : Poly1305_amd64_5xPR.M.carry_reduce_u128 ~ Poly1305_avx_5x.M.carry_reduce_u128 : 
         rela5 hx{1} hy{1} x{2} ==>
@@ -240,12 +266,9 @@ equiv carry_reduce_u128P : Poly1305_amd64_5xPR.M.carry_reduce_u128 ~ Poly1305_av
 proof.
   conseq (_: rela5 res{1}.`1 res{1}.`2 res{2}) (_ : true ==> wf5 res.`1 /\ wf5 res.`2) => //.
   + by proc; do 2!call carry_reduceWF;auto.
-  proc; inline *; wp; skip; cbv delta.
+  proc. inline *. wp; skip;rewrite /rela5 => /=. 
   move=> &m1 &m2 [#] 5!->. cbv delta.  
-  rewrite (zeroext_bounded (hx{m1}.[4] + (hx{m1}.[3] `>>>` 26) `>>>` 26)) //.
-  admit.    (* 57 *)
-  rewrite (zeroext_bounded (hy{m1}.[4] + (hy{m1}.[3] `>>>` 26) `>>>` 26)) //.
-  admit.    (* 57 *)
+  by rewrite -!zeroext_and2p32.
 qed.
 
 hoare clampWF : Poly1305_amd64_5xPR.M.clamp : true ==> wf5 res.
@@ -283,6 +306,8 @@ proof.
   by unroll for {2} 5; wp; skip => &m1 &m2; cbv delta => [#] 5!->.
 qed.
 
+axiom zeroext_bounded w : bounded 32 w => zeroext_32_64 (unpack_2u32 w).`1 = w.
+ 
 equiv mulmod_u128P : 
   Poly1305_amd64_5xPR.M.mulmod_u128 ~ Poly1305_avx_5x.M.mulmod_u128 : 
   wf5 x1{1} /\ wf5 x2{1} /\ wf5 y1{1} /\ wf5 y2{1} /\ wf4 y1x5{1} /\ wf4 y2x5{1} /\
@@ -295,37 +320,7 @@ proof.
   move=> &m1 &m2 [#] X10 X11 X12 X13 X14 X20 X21 X22 X23 X24.
   move=> Y10 Y11 Y12 Y13 Y14 Y20 Y21 Y22 Y23 Y24.
   move=> Y1x0 Y1x1 Y1x2 Y1x3 Y2x0 Y2x1 Y2x2 Y2x3 14!-> /=.
-  rewrite (zeroext_bounded x1{m1}.[0]); 1:by move: X10;apply: bounded_weak.
-  rewrite (zeroext_bounded x1{m1}.[1]); 1:by move: X11;apply: bounded_weak.
-  rewrite (zeroext_bounded x1{m1}.[2]); 1:by move: X12;apply: bounded_weak.
-  rewrite (zeroext_bounded x1{m1}.[3]); 1:by move: X13;apply: bounded_weak.
-  rewrite (zeroext_bounded x1{m1}.[4]); 1:by move: X14;apply: bounded_weak.
-  rewrite (zeroext_bounded x2{m1}.[0]); 1:by move: X20;apply: bounded_weak.
-  rewrite (zeroext_bounded x2{m1}.[1]); 1:by move: X21;apply: bounded_weak.
-  rewrite (zeroext_bounded x2{m1}.[2]); 1:by move: X22;apply: bounded_weak.
-  rewrite (zeroext_bounded x2{m1}.[3]); 1:by move: X23;apply: bounded_weak.
-  rewrite (zeroext_bounded x2{m1}.[4]); 1:by move: X24;apply: bounded_weak.
-
-  rewrite (zeroext_bounded y1{m1}.[0]); 1:by move: Y10;apply: bounded_weak.
-  rewrite (zeroext_bounded y1{m1}.[1]); 1:by move: Y11;apply: bounded_weak.
-  rewrite (zeroext_bounded y1{m1}.[2]); 1:by move: Y12;apply: bounded_weak.
-  rewrite (zeroext_bounded y1{m1}.[3]); 1:by move: Y13;apply: bounded_weak.
-  rewrite (zeroext_bounded y1{m1}.[4]); 1:by move: Y14;apply: bounded_weak.
-  rewrite (zeroext_bounded y2{m1}.[0]); 1:by move: Y20;apply: bounded_weak.
-  rewrite (zeroext_bounded y2{m1}.[1]); 1:by move: Y21;apply: bounded_weak.
-  rewrite (zeroext_bounded y2{m1}.[2]); 1:by move: Y22;apply: bounded_weak.
-  rewrite (zeroext_bounded y2{m1}.[3]); 1:by move: Y23;apply: bounded_weak.
-  rewrite (zeroext_bounded y2{m1}.[4]); 1:by move: Y24;apply: bounded_weak.
-
-  rewrite (zeroext_bounded y1x5{m1}.[0]); 1:by move: Y1x0;apply: bounded_weak.
-  rewrite (zeroext_bounded y1x5{m1}.[1]); 1:by move: Y1x1;apply: bounded_weak.
-  rewrite (zeroext_bounded y1x5{m1}.[2]); 1:by move: Y1x2;apply: bounded_weak.
-  rewrite (zeroext_bounded y1x5{m1}.[3]); 1:by move: Y1x3;apply: bounded_weak.
-  rewrite (zeroext_bounded y2x5{m1}.[0]); 1:by move: Y2x0;apply: bounded_weak.
-  rewrite (zeroext_bounded y2x5{m1}.[1]); 1:by move: Y2x1;apply: bounded_weak.
-  rewrite (zeroext_bounded y2x5{m1}.[2]); 1:by move: Y2x2;apply: bounded_weak.
-  rewrite (zeroext_bounded y2x5{m1}.[3]); 1:by move: Y2x3;apply: bounded_weak.
-  done.
+  smt (zeroext_bounded bounded_weak).
 qed.
 
 equiv mulmod_add_u128P : 
@@ -343,28 +338,7 @@ proof.
   wp; skip; cbv delta.
   move=> &m1 &m2 [#] X10 X11 X12 X13 X14 X20 X21 X22 X23 X24.
   move=> Y0 Y1 Y2 Y3 Y4 Yx0 Yx1 Yx2 Yx3 19!-> /=.
-  rewrite (zeroext_bounded x1{m1}.[0]); 1:by move: X10;apply: bounded_weak.
-  rewrite (zeroext_bounded x1{m1}.[1]); 1:by move: X11;apply: bounded_weak.
-  rewrite (zeroext_bounded x1{m1}.[2]); 1:by move: X12;apply: bounded_weak.
-  rewrite (zeroext_bounded x1{m1}.[3]); 1:by move: X13;apply: bounded_weak.
-  rewrite (zeroext_bounded x1{m1}.[4]); 1:by move: X14;apply: bounded_weak.
-  rewrite (zeroext_bounded x2{m1}.[0]); 1:by move: X20;apply: bounded_weak.
-  rewrite (zeroext_bounded x2{m1}.[1]); 1:by move: X21;apply: bounded_weak.
-  rewrite (zeroext_bounded x2{m1}.[2]); 1:by move: X22;apply: bounded_weak.
-  rewrite (zeroext_bounded x2{m1}.[3]); 1:by move: X23;apply: bounded_weak.
-  rewrite (zeroext_bounded x2{m1}.[4]); 1:by move: X24;apply: bounded_weak.
-
-  rewrite (zeroext_bounded y{m1}.[0]); 1:by move: Y0;apply: bounded_weak.
-  rewrite (zeroext_bounded y{m1}.[1]); 1:by move: Y1;apply: bounded_weak.
-  rewrite (zeroext_bounded y{m1}.[2]); 1:by move: Y2;apply: bounded_weak.
-  rewrite (zeroext_bounded y{m1}.[3]); 1:by move: Y3;apply: bounded_weak.
-  rewrite (zeroext_bounded y{m1}.[4]); 1:by move: Y4;apply: bounded_weak.
- 
-  rewrite (zeroext_bounded yx5{m1}.[0]); 1:by move: Yx0;apply: bounded_weak.
-  rewrite (zeroext_bounded yx5{m1}.[1]); 1:by move: Yx1;apply: bounded_weak.
-  rewrite (zeroext_bounded yx5{m1}.[2]); 1:by move: Yx2;apply: bounded_weak.
-  rewrite (zeroext_bounded yx5{m1}.[3]); 1:by move: Yx3;apply: bounded_weak.
-  done.
+  smt (zeroext_bounded bounded_weak).
 qed.
 
 equiv add_u128P : Poly1305_amd64_5xPR.M.add_u128 ~ Poly1305_avx_5x.M.add_u128 :  
@@ -392,9 +366,11 @@ proof.
   conseq (_: ={global_mem} /\ in_0{1} = m{2} ==> rela5 res{1}.`1 res{1}.`2 res{2}) 
          (_: true ==> wf5 res.`1 /\ wf5 res.`2).
   + by proc; do !(call loadWF;wp); skip.
-  proc;inline *;wp; skip => />; cbv delta.
-
-
+  proc;inline *;wp; skip => />; cbv delta => &1.
+  rewrite !W64_addw0 -!W64_addwA W64_addi /= !W64_shr_add //=.
+  rewrite !W64_shr_or !W64_shr_add //= !(W64_shr_64 78) //= !W64_or0w.
+  admit. (* it is true since we look only on the low bit *)
+qed.
 
 equiv remaining_blocksP : Poly1305_amd64_5xPR.M.remaining_blocks ~ Poly1305_avx_5x.M.remaining_blocks :
    ={global_mem, in_0} /\ 
@@ -404,32 +380,33 @@ equiv remaining_blocksP : Poly1305_amd64_5xPR.M.remaining_blocks ~ Poly1305_avx_
    rela5 s_r4{1} s_r4{1} s_r4r4{2} /\ 
    rela4 s_r2x5{1} s_r2x5{1} s_r2r2x5{2} /\
    rela4 s_r4x5{1} s_r4x5{1} s_r4r4x5{2} ==>
-   res{1}.`3 = res{2}.`2 /\
+   res{1}.`3 = res{2}.`2 /\ wf5 res{1}.`1 /\ wf5 res{1}.`2 /\
    rela5 res{1}.`1 res{1}.`2 res{2}.`1.
 proof.
   proc => /=.
-  call carry_reduce_u128P. (* need precondition 57 *)
-  call add_u128P;wp. (* need precondition 56 *)  
-  
- 
-  
-  
-
-
-  swap{1}16 9. swap{1} 15 8; wp.
-  seq 22 9 : (#post). 
-  + admit.
-  inline *.
-  wp; skip; cbv delta => &m1 &m2 [#] 5!->; cbv delta.
-admitted.
+  call carry_reduce_u128P. 
+  call add_u128P; wp. 
+  call unpack_u128P.
+  call mulmod_add_u128P; wp.
+  call unpack_u128P.
+  by call mulmod_u128P; wp; skip.
+qed.
 
 equiv first_blockP : Poly1305_amd64_5xPR.M.first_block ~ Poly1305_avx_5x.M.first_block :
    ={global_mem, in_0} /\
+   wf5 s_r2{1} /\ wf4 s_r2x5{1} /\
    rela5 s_r2{1} s_r2{1} s_r2r2{2} /\
    rela4 s_r2x5{1} s_r2x5{1} s_r2r2x5{2} ==>
    res{1}.`3 = res{2}.`2 /\
-   rela5 res{1}.`1 res{1}.`2 res{2}.`1.
-admitted.
+   rela5 res{1}.`1 res{1}.`2 res{2}.`1 /\ wf5 res{1}.`1 /\ wf5 res{1}.`2.
+proof.
+  proc => /=.
+  call carry_reduce_u128P.
+  call add_u128P; wp.
+  call unpack_u128P; wp.
+  call mulmod_u128P; wp.
+  by call unpack_u128P; wp; skip.
+qed.
 
 equiv final_mulP : Poly1305_amd64_5xPR.M.final_mul ~ Poly1305_avx_5x.M.final_mul : 
   wf5 hx{1} /\ wf5 hy{1} /\ wf5 s_r2{1} /\ wf4 s_r2x5{1} /\ wf5 s_r{1} /\ wf4 s_rx5{1} /\
@@ -440,7 +417,7 @@ proof.
   proc => /=.
   call hadd_u128P => /=.
   call carry_reduce_u128P.
-  call mulmod_u128P.  (* We need to ensure bounded 57 hx.[3] hx.[4] hy.[3] hy.[4] *)
+  call mulmod_u128P.  
   by wp; skip => />.
 qed.
 
@@ -465,7 +442,7 @@ equiv poly1305_amd64_avx_5x :
 proof.
   proc=> /=. sim.
   seq 20 26 : 
-    (#pre /\ (r=s_r){1} /\ bounded_32_5 r{1} /\
+    (#pre /\ (r=s_r){1} /\ wf5 r{1} /\
     ={s_out, s_in, s_inlen, s_k, r, s_r, s_rx5, s_r2x5, h}).
   + wp. call clampP => /=. 
     conseq (_ :
@@ -474,16 +451,19 @@ proof.
   seq 2 2 : (#pre /\  (is_x5 r s_rx5){1}).
   + conseq />;unroll for {1} 2; unroll for {2} 2.
     by wp;skip;cbv delta => />.
-  seq 4 4 : (#pre /\ ={b64}).
-  + by sim />.
+  seq 0 0 : (#pre /\ wf4 s_rx5{1}).
+  + by skip => &m1 &m2 /> R0 R1 R2 R3 R4 4!->; rewrite !bounded_mul5.
+  seq 4 4 : (#pre /\ ={b64}); 1: by sim />.
   if => //.
   seq 0 0 : (#[/:-1]pre); 1: by auto. 
-  seq 5 5 : (#pre /\ ={r2, s_b64, s_r2} /\ (r2 = s_r2){1} /\ bounded_32_5 r2{1}).
+  seq 5 5 : (#pre /\ ={r2, s_b64, s_r2} /\ (r2 = s_r2){1} /\ wf5 r2{1}).
   + conseq |>; wp; call carry_reduceP.
     by conseq (_: ={r2, s_b64}) => //; sim.
   seq 2 2 : (#pre /\ (is_x5 r2 s_r2x5){1}).
   + conseq />;unroll for {1} 2; unroll for {2} 2.
     by wp;skip;cbv delta => />.
+  seq 0 0 : (#pre /\ wf4 s_r2x5{1}).
+  + by skip => &m1 &m2 |> ? ? ? />  R0 R1 R2 R3 R4 4!->; rewrite !bounded_mul5.
   seq 0 1 : (#pre); 1: by auto.
   seq 0 2 : (#pre /\ (r2r = s_r2r){2} /\ rela5 r2{1} r{1} r2r{2}).
   + wp.
@@ -491,38 +471,38 @@ proof.
     by call{2} (unpack_u26x5x2P r2_R r_R); skip => />.
   seq 0 2 : (#pre /\ rela4 s_r2x5{1} s_rx5{1} s_r2rx5{2}).
   + conseq />;unroll for {2} 2.
-    wp;skip => /> &m2 ????? 4!-> ????? 4!-> ? 4!->.
-    cbv delta.
-    rewrite (zeroext_bounded s_r2{m2}.[1]) // (zeroext_bounded s_r2{m2}.[2]) //.
-    rewrite (zeroext_bounded s_r2{m2}.[3]) // (zeroext_bounded s_r2{m2}.[4]) //.
-    rewrite (zeroext_bounded s_r{m2}.[1]) // (zeroext_bounded s_r{m2}.[2]) //.
-    by rewrite (zeroext_bounded s_r{m2}.[3]) // (zeroext_bounded s_r{m2}.[4]).
+    wp;skip => |> &m2 + + _ + + _.
+    move=> /> R0 R1 R2 R3 R4 4!-> R20 R21 R22 R23 R24 4!->  ? 4!->.
+    cbv delta; smt (zeroext_bounded bounded_weak).
   seq 0 2 : (#pre /\ (r2r2 = s_r2r2){2} /\ rela5 r2{1} r2{1} r2r2{2}).
   + wp; conseq />.
     exists * r2{2}; elim * => r2_R.
     by call{2} (unpack_u26x5x2P r2_R r2_R); skip => />.
   seq 0 2 : (#pre /\ rela4 s_r2x5{1} s_r2x5{1} s_r2r2x5{2}).
   + conseq />;unroll for {2} 2.
-    wp;skip => /> &m2 ????? 4!-> ????? 4!-> ????? ???? ? 4!->.
-    cbv delta.
-    rewrite (zeroext_bounded s_r2{m2}.[1]) // (zeroext_bounded s_r2{m2}.[2]) //.
-    by rewrite (zeroext_bounded s_r2{m2}.[3]) // (zeroext_bounded s_r2{m2}.[4]).
+    wp;skip => |> &m _ _ _ + + _ _ _.
+    move=> /> ?????  4!-> ? 4!->.  
+    cbv delta; smt (zeroext_bounded bounded_weak).
   seq 1 1 : (#pre /\ (b64 = s_b64){1}); 1: by auto. 
   if => //.
-  + seq 4 3 : (#pre /\ ={r4} /\ (r4 = s_r4){1} /\ bounded_32_5 r4{1}).
-      + conseq |>; wp;call carry_reduceP.
-        by conseq (_: ={r4}) => //; sim.
-      seq 0 2 : (#pre /\ (r4r4=s_r4r4){2} /\ rela5 r4{1} r4{1} r4r4{2}).
-      + wp; exists * r4{2}; elim * => r4_R.
+  + seq 4 3 : (#pre /\ ={r4} /\ (r4 = s_r4){1} /\ wf5 r4{1}).
+    + conseq |>; wp;call carry_reduceP.
+      by conseq (_: ={r4}) => //; sim.
+    seq 0 2 : (#pre /\ (r4r4=s_r4r4){2} /\ rela5 r4{1} r4{1} r4r4{2}).
+    + wp; exists * r4{2}; elim * => r4_R.
       by call{2} (unpack_u26x5x2P r4_R r4_R); skip => />.
-    seq 2 2 : (#pre /\ rela4 s_r4x5{1} s_r4x5{1} s_r4r4x5{2}).
+    seq 2 2 : (#pre /\ is_x5 r4{1} s_r4x5{1} /\ rela4 s_r4x5{1} s_r4x5{1} s_r4r4x5{2}).
     + unroll for {1} 2. unroll for {2} 2.
-      wp; skip => /> &m1 &m2 ????? ???? ????? ???? ????? ???? ????? ???? ? ????? ? 4!->.
-      cbv delta.
-      rewrite (zeroext_bounded s_r4{m1}.[1]) // (zeroext_bounded s_r4{m1}.[2]) //.
-      by rewrite (zeroext_bounded s_r4{m1}.[3]) // (zeroext_bounded s_r4{m1}.[4]).
-    call final_mulP; conseq (_ : rela5 hx{1} hy{1} hxy{2} /\ ={in_0}) => //.
+      wp; skip => |> &m1 &m2 _ _ _ _ _ _ _ _ _ _ _ /> ????? ? 4!->. 
+      cbv delta; smt (zeroext_bounded bounded_weak).
+    seq 0 0 : (#pre /\ wf4 s_r4x5{1}).
+    + skip => &m1 &m2 |> ??????????? + _ + _.
+      by move=> /> ????? 4!->; rewrite !bounded_mul5.
+    call final_mulP => /=.
     while (={global_mem, b64, in_0} /\ 
+            wf5 hx{1}   /\ wf5 hy{1} /\
+            wf5 s_r2{1} /\ wf4 s_r2x5{1} /\
+            wf5 s_r4{1} /\ wf4 s_r4x5{1} /\
             rela5 hx{1} hy{1} hxy{2} /\ 
             rela5 s_r2{1} s_r2{1} s_r2r2{2} /\ 
             rela5 s_r4{1} s_r4{1} s_r4r4{2} /\ 
@@ -532,11 +512,11 @@ proof.
     by wp; call first_blockP; wp; skip.  
   rcondf{1} 5.  
   + move=> &m2; wp; conseq (_: true) => //.
-    move=> |> ????????. admit. (* would be simpler if we use unsigned comparison *)
+    move=> |> ??????????. 
+    admit. (* fact on comparison *)
   rcondf{2} 5.
   + move=> &m1; wp; conseq (_: true) => //.
-    move=> |> ????????.  admit. (* would be simpler if we use unsigned comparison *) 
-  call final_mulP; conseq (_ : rela5 hx{1} hy{1} hxy{2} /\ ={in_0}) => //.
-  by wp; call first_blockP; wp; skip.  
+    move=> |> ???????????.  admit. 
+  by call final_mulP; wp; call first_blockP; wp; skip.  
 qed.
 
